#############################
# MSO-EM epistemic ontology #
#############################

@base <https://www.purl.org/mso-em#>.
@prefix mso-em: <https://www.purl.org/mso-em#>.

@prefix dcelem: <http://purl.org/dc/elements/1.1/>.
@prefix dcterms: <http://purl.org/dc/terms/>.
@prefix dol: <http://www.loa-cnr.it/ontologies/DOLCE-Lite.owl#>.
@prefix ineurese: <http://purl.org/info:eu-repo/semantics/>.
@prefix pims-ii: <http://www.molmod.info/semantics/pims-ii.ttl#>.
@prefix skos: <http://www.w3.org/2004/02/skos/core#>.
@prefix vann: <http://purl.org/vocab/vann/>.
@prefix xs: <http://www.w3.org/2001/XMLSchema#>.

<https://www.purl.org/mso-em-epistemic> a owl:Ontology;
   owl:versionIRI <https://batcat.info/semantics/mso-em-2024-12/epistemic.ttl>;
   dcterms:title "MSO-EM module 'epistemic' (Assessment, KnowledgeClaim, ValidityClaim)"^^xs:string;
   dcterms:created "2024"^^dcterms:W3CDTF;
   owl:versionInfo "MSO-EM module 'epistemic': Version dated July 2025"^^xs:string;
   dcterms:issued "2025-07-18"^^dcterms:W3CDTF;
   dcterms:publisher "BatCAT consortium (Horizon Europe GA no. 101137725)"^^xs:string;
   dcterms:license <https://creativecommons.org/licenses/by-nd/4.0/>;
   dcterms:creator <https://orcid.org/0000-0002-9464-6739>;  # Martin Thomas Horsch
   dcterms:status ineurese:publishedVersion;
   dcterms:source <http://www.molmod.info/semantics/pims-ii.ttl>;
   vann:preferredNamespaceUri "https://www.purl.org/mso-em#"^^xs:string;
   dcelem:description "MSO-EM module for epistemic. Its highest-level concepts are Assessment, KnowledgeClaim, and ValidityClaim."@en;
   dcterms:bibliographicCitation "M. T. Horsch, S. Chiacchiera, I. T. Todorov, A. T. Correia, A. Dey, N. A. Konchakova, S. Scholze, S. Stephan, K. Tøndel, A. Sarkar, M. H. Karray, F. Al Machot, B. Schembera, 'Exploration of key concepts required for mid- and domain-level ontology development to facilitate explainable-AI-readiness of data and models,' submitted, 2024."@en.


##########################
# Highest-level concepts #
##########################

mso-em:Assessment a owl:Class;
   skos:prefLabel "assessment"@en;
   skos:altLabel  "Assessment"@en;
   rdfs:subClassOf dol:proposition, [
         a owl:Restriction;
         owl:onProperty mso-em:isAbout;
         owl:someValuesFrom mso-em:Cognition
      ];
   skos:exactMatch pims-ii:Assessment;
   skos:definition "ground that provides an explanation including a proposition on the extent (quantitatively or qualitatively) to which the grounded cognition is reliable, accurate, valid, or similar, and why that is the case"@en.

mso-em:KnowledgeClaim a owl:Class;
   skos:prefLabel "knowledge claim"@en;
   skos:altLabel  "KnowledgeClaim"@en;
   rdfs:subClassOf mso-em:Claim, dol:proposition, [
         a owl:Restriction;
         owl:onProperty mso-em:isBasedOn;
         owl:someValuesFrom mso-em:Articulation
      ];
   owl:disjointWith mso-em:ValidityClaim;
   skos:exactMatch pims-ii:KnowledgeClaim;
   skos:definition "claim asserting the knowledge status of something / proposition asserting the knowledge status of another proposition"@en;
   skos:scopeNote "The subject matter of a knowledge claim must be a (single) question, namely the one that is answered by the claim; in particular, therefore, its subject matter may not be a sum (plurality) of unrelated questions - in such a case, split it up into multiple independent knowledge claims"@en;
   skos:scopeNote "A knowledge claim states 'what data mean,' i.e., in what way some agent of the academic discourse has given some data an interpretation as constituting knowledge. A knowledge claim asserts what was found from research data: 'Research data δ made agent a know φ,' which can be expanded as 'the interpreation of research data δ by interpreter a yielded the knowledge claim φ as an interpretant.'"@en.

mso-em:ValidityClaim a owl:Class;
   skos:prefLabel "validity claim"@en;
   skos:altLabel  "ValidityClaim"@en;
   rdfs:subClassOf mso-em:Claim, [
          a owl:Restriction;
          owl:onProperty;
          owl:someValuesFrom mso-em:Claim
      ];
   owl:disjointWith mso-em:KnowledgeClaim;
   skos:exactMatch pims-ii:ValidityClaim;
   skos:definition "claim about another claim, saying something about that claim's (in-)accuracy or somebody's (dis-)trust in the claim"@en.


############################################
# Properties of the highest-level concepts #
############################################



############################
# Subclasses of Assessment #
############################



##########################################
# Properties of subclasses of Assessment #
##########################################



################################
# Subclasses of KnowledgeClaim #
################################



##############################################
# Properties of subclasses of KnowledgeClaim #
##############################################



###############################
# Subclasses of ValidityClaim #
###############################



#############################################
# Properties of subclasses of ValidityClaim #
#############################################

