############################
# MSO-EM quantity ontology #
############################

@base <https://www.purl.org/mso-em#>.
@prefix mso-em: <https://www.purl.org/mso-em#>.

@prefix dcelem: <http://purl.org/dc/elements/1.1/>.
@prefix dcterms: <http://purl.org/dc/terms/>.
@prefix dol: <http://www.loa-cnr.it/ontologies/DOLCE-Lite.owl#>.
@prefix ineurese: <http://purl.org/info:eu-repo/semantics/>.
@prefix pims-ii: <http://www.molmod.info/semantics/pims-ii.ttl#>.
@prefix skos: <http://www.w3.org/2004/02/skos/core#>.
@prefix vann: <http://purl.org/vocab/vann/>.
@prefix xs: <http://www.w3.org/2001/XMLSchema#>.

<https://www.purl.org/mso-em-quantity> a owl:Ontology;
   owl:versionIRI <https://batcat.info/semantics/mso-em-2025-07/quantity.ttl>;
   dcterms:title "MSO-EM module 'quantity' (Equation, Term, Unit)"@en;
   dcterms:created "2025"^^dcterms:W3CDTF;
   owl:versionInfo "MSO-EM module 'quantity': Version dated July 2025"@en;
   dcterms:issued "2025-07-13"^^dcterms:W3CDTF;
   dcterms:publisher "BatCAT consortium (Horizon Europe GA no. 101137725)"@en;
   dcterms:license <https://creativecommons.org/licenses/by-nd/4.0/>;
   dcterms:creator <https://orcid.org/0000-0002-9464-6739>;  # Martin Thomas Horsch
   dcterms:status ineurese:publishedVersion;
   dcterms:source <http://www.molmod.info/semantics/pims-ii.ttl>;
   vann:preferredNamespaceUri "https://www.purl.org/mso-em#"^^xs:string;
   dcelem:description "MSO-EM module for quantities. Its highest-level concepts are Equation, Term, and Unit."@en;
   dcterms:bibliographicCitation "M. T. Horsch, S. Chiacchiera, I. T. Todorov, A. T. Correia, A. Dey, N. A. Konchakova, S. Scholze, S. Stephan, K. TÃ¸ndel, A. Sarkar, M. H. Karray, F. Al Machot & B. Schembera (2024). Exploration of core concepts required for mid- and domain-level ontology development to facilitate explainable-AI-readiness of data and models. In R. Confalonieri et al. (editors), Data meets Ontologies in Explainable AI 2024: 5. CEUR-WS, Aachen."@en.


##########################
# Highest-level concepts #
##########################

mso-em:Equation a owl:Class;
   skos:prefLabel "equation"@en;
   skos:altLabel  "Equation"@en;
   rdfs:subClassOf mso-em:Dyad, dol:non-physical-endurant, [
      a owl:Restriction;
      owl:onProperty mso-em:hasLeftEntry;
      owl:someValuesFrom mso-em:Term
   ], [
      a owl:Restriction;
      owl:onProperty mso-em:hasRightEntry;
      owl:someValuesFrom mso-em:Term
   ];
   skos:exactMatch pims-ii:EqualityArticulation;
   skos:definition "dyad by which two terms are asserted to be equal or to become equal"@en.

mso-em:Term a owl:Class;
   skos:prefLabel "term"@en;
   skos:altLabel  "Term"@en;
   rdfs:subClassOf mso-em:Articulation, dol:non-physical-endurant, [
      a owl:Restriction;
      owl:onProperty mso-em:represents;
      owl:someValuesFrom owl:Thing
   ];
   skos:exactMatch pims-ii:Term;
   skos:definition "conventional articulation that can evaluate to a value"@en;
   skos:scopeNote "terms include variables, values, and any mathematically and semantically valid ways of combining variables, values, and mathematical operators - note that it is required for a term to potentially take a value"@en.

mso-em:Unit a owl:Class;
   skos:prefLabel "unit"@en;
   skos:altLabel  "Unit"@en;
   rdfs:subClassOf mso-em:Literal, dol:non-physical-endurant;
   skos:exactMatch pims-ii:MeasurementUnit;
   skos:definition "'real scalar quantity, defined and adopted by convention' (EMMO, ISO 80000-1)"@en.


############################################
# Properties of the highest-level concepts #
############################################

mso-em:hasAdmissibleUnit a owl:ObjectProperty;
   skos:prefLabel "has admissible unit"@en;
   skos:altLabel "hasAdmissibleUnit"@en;
   rdfs:domain mso-em:Term;
   rdfs:range mso-em:Unit;
   rdfs:subPropertyOf dol:generic-constituent;
   skos:definition "(x has admissible unit y) means that x is a term that, in principle, can take values with the unit y"@en.

mso-em:hasValue a owl:ObjectProperty;
   skos:prefLabel "has value"@en;
   skos:altLabel "hasValue"@en;
   rdfs:domain mso-em:Term;
   rdfs:range mso-em:Value;
   rdfs:subPropertyOf mso-em:represents;
   skos:definition "(x has value y) means that x is a term, and y is its value"@en.


##########################
# Subclasses of Equation #
##########################

mso-em:Assignment a owl:Class;
   skos:prefLabel "assignment"@en;
   skos:altLabel "Assignment"@en;
   rdfs:subClassOf mso-em:Equation, [
      a owl:Restriction;
      owl:onProperty mso-em:assignsTo;
      owl:someValuesFrom mso-em:Variable
   ], [
      a owl:Restriction;
      owl:onProperty mso-em:assignsValueOf;
      owl:someValuesFrom mso-em:Term
   ];
   skos:exactMatch pims-ii:Assignment;
   skos:definition "equality articulation by which a value is assigned to a variable with respect to a particular referent"@en;
   skos:example "e.g., T = 200 K for substance o as it was measured in a particular cognitive step; therein, T is the variable, related to the assignment by 'assigns to,' 200 K is the value, related to the assignment by 'assigns value of,' and o is the referent, related to the assignment by 'assigns for referent'."@en.


########################################
# Properties of subclasses of Equation #
########################################

mso-em:assignsForReferent a owl:ObjectProperty;
   skos:prefLabel "assigns for referent"@en;
   skos:altLabel "assignsForReferent"@en;
   rdfs:domain mso-em:Assignment;
   rdfs:subPropertyOf mso-em:isAbout;
   skos:definition "(a assigns for referent o) means that a: x = y is an assignment that is about the object o, wherein x represents o"@en;
   skos:example "e.g., x may be thermodynamic temperature, y may be a temperature value, and o may be an object of which the temperature has been measured"@en.

mso-em:assignsTo a owl:ObjectProperty;
   skos:prefLabel "assigns to"@en;
   skos:altLabel "assignsTo"@en;
   rdfs:domain mso-em:Assignment;
   rdfs:range mso-em:Variable;
   rdfs:subPropertyOf mso-em:hasLeftEntry;
   skos:definition "(a assigns to x) means that a: x = y is an assignment where the value of the term y is assigned to a variable x"@en.

mso-em:assignsValueOf a owl:ObjectProperty;
   skos:prefLabel "assigns value of"@en;
   skos:altLabel "assignsValueOf"@en;
   rdfs:domain mso-em:Assignment;
   rdfs:range mso-em:Term;
   rdfs:subPropertyOf mso-em:hasRightEntry;
   skos:definition "(a assigns value of y) means that a: x = y is an assignment where the value of the term y is assigned to a variable x"@en.


######################
# Subclasses of Term #
######################

mso-em:Property a owl:Class;
   skos:prefLabel "property"@en;
   skos:altLabel "Property"@en;
   rdfs:subClassOf mso-em:Variable;
   skos:exactMatch pims-ii:Property;
   skos:definition "variable that is employed for the possible outcome of observations and similar processes"@en.

mso-em:QuantityValue a owl:Class;
   skos:prefLabel "quantity value"@en;
   skos:altLabel "QuantityValue"@en;
   rdfs:subClassOf mso-em:Value;
   owl:equivalentClass [
      owl:intersectionOf (
         [
            a owl:Restriction;
            owl:onProperty mso-em:hasMagnitude;
            owl:someValuesFrom mso-em:Literal
         ] [
            a owl:Restriction;
            owl:onProperty mso-em:hasUnit;
            owl:someValuesFrom mso-em:Unit
         ]
      )
   ];
   skos:exactMatch pims-ii:QuantityValue;
   skos:definition "value that has a numerical magnitude and a physical unit"@en.

mso-em:Value a owl:Class;
   skos:prefLabel "value"@en;
   skos:altLabel  "Value"@en;
   rdfs:subClassOf mso-em:Term;
   skos:exactMatch pims-ii:Term;
   skos:definition "articulation that is by social convention understood to be potentially assignable to a variable"@en.

mso-em:Variable a owl:Class;
   skos:prefLabel "variable"@en;
   skos:altLabel "Variable"@en;
   rdfs:subClassOf mso-em:Term;
   skos:exactMatch pims-ii:Variable;
   skos:definition "conventional that is employed for something to which values can be assigned"@en;
   skos:scopeNote "this is to be understood very generally, e.g., a variable may be an array or set of elements or have another kind of internal structure"@en.


####################################
# Properties of subclasses of Term #
####################################

mso-em:hasMagnitude a owl:ObjectProperty;
   skos:prefLabel "has magnitude"@en;
   skos:altLabel "hasMagnitude"@en;
   rdfs:domain mso-em:Value;
   rdfs:range mso-em:Literal;
   rdfs:subPropertyOf mso-em:hasEntry;
   skos:definition "(x has magnitude y) means that x is the numerical magnitude of the value y"@en;
   skos:example "e.g., in 200 kPa, the magnitude would be the literal 200, i.e., a mso-em:Literal object that mso-em:isLiterally the XSD/RDF literal 200"@en.

mso-em:hasUnit a owl:ObjectProperty;
   skos:prefLabel "has unit"@en;
   skos:altLabel "hasUnit"@en;
   rdfs:domain mso-em:Value;
   rdfs:range mso-em:Unit;
   rdfs:subPropertyOf mso-em:hasEntry;
   skos:definition "(x has unit y) means that x is the unit of the value y"@en;
   skos:example "e.g., in 200 kPa, the unit would be kPa"@en.
