#############################
# MSO-EM semiotics ontology #
#############################

@base <https://www.purl.org/mso-em#>.
@prefix mso-em: <https://www.purl.org/mso-em#>.

@prefix dcelem: <http://purl.org/dc/elements/1.1/>.
@prefix dcterms: <http://purl.org/dc/terms/>.
@prefix dol: <http://www.loa-cnr.it/ontologies/DOLCE-Lite.owl#>.
@prefix ineurese: <http://purl.org/info:eu-repo/semantics/>.
@prefix pims-ii: <http://www.molmod.info/semantics/pims-ii.ttl#>.
@prefix skos: <http://www.w3.org/2004/02/skos/core#>.
@prefix vann: <http://purl.org/vocab/vann/>.
@prefix xs: <http://www.w3.org/2001/XMLSchema#>.

<https://www.purl.org/mso-em-semiotics> a owl:Ontology;
   owl:versionIRI <https://batcat.info/semantics/mso-em-2024-10/semiotics.ttl>;
   dcterms:title "MSO-EM module 'semiotics' (Claim, Cognition, Communication)"^^xs:string;
   dcterms:created "2024"^^dcterms:W3CDTF;
   owl:versionInfo "MSO-EM module 'semiotics': Version dated October 2024"^^xs:string;
   dcterms:issued "2024-10-25"^^dcterms:W3CDTF;
   dcterms:publisher "BatCAT consortium (Horizon Europe GA no. 101137725)"^^xs:string;
   dcterms:license <https://creativecommons.org/licenses/by-nd/4.0/>;
   dcterms:creator <https://orcid.org/0000-0002-9464-6739>;  # Martin Thomas Horsch
   dcterms:status ineurese:publishedVersion;
   dcterms:source <http://www.molmod.info/semantics/pims-ii.ttl>;
   vann:preferredNamespaceUri "https://www.purl.org/mso-em#"^^xs:string;
   dcelem:description "MSO-EM module for semiotics. Its highest-level concepts are Claim, Cognition, and Communication."@en;
   dcterms:bibliographicCitation "M. T. Horsch, S. Chiacchiera, I. T. Todorov, A. T. Correia, A. Dey, N. A. Konchakova, S. Scholze, S. Stephan, K. TÃ¸ndel, A. Sarkar, M. H. Karray, F. Al Machot, B. Schembera, 'Exploration of key concepts required for mid- and domain-level ontology development to facilitate explainable-AI-readiness of data and models,' submitted, 2024."@en.


##########################
# Highest-level concepts #
##########################

mso-em:Claim a owl:Class;
   skos:prefLabel "claim"@en;
   skos:altLabel  "Claim"@en;
   rdfs:subClassOf dol:proposition;
   owl:equivalentClass [
      a owl:Restriction;
      owl:onProperty mso-em:isAssertedBy;
      owl:someValuesFrom mso-em:Interlocutor
   ];
   owl:disjointWith mso-em:Question;
   skos:exactMatch pims-ii:Claim;
   skos:definition "proposition that is asserted by an interlocutor"@en.

mso-em:Cognition a owl:Class;
   skos:prefLabel "cognition"@en;
   skos:altLabel  "Cognition"@en;
   rdfs:subClassOf mso-em:Action;
   skos:exactMatch pims-ii:Cognition;
   skos:definition "process dealing with signs and the representation of objects by signs"@en;
   skos:scopeNote "The congition can consist of a single cognitive step or of multiple steps that are connected to each other as a cognitive chain"@en;
   skos:editorialNote "Now subsumed under action; this is a change from PIMS-II where it was possible for a cognition not to be an action"@en.

mso-em:Communication a owl:Class;
   skos:prefLabel "communication"@en;
   skos:altLabel  "Communication"@en;
   rdfs:subClassOf mso-em:PurposefulAction, [
      a owl:Restriction;
      owl:onProperty dol:part;
      owl:someValuesFrom mso-em:ExpressiveAct
   ];
   skos:exactMatch pims-ii:Communication;
   skos:definition "purposeful action wherein multiple interlocutors engage in an exchange of information with another"@en;
   skos:scopeNote "A communication involves at least one expressive act. The agent here includes all those who are speaking; i.e., it can be a group of people (not necessarily therefore an interlocutor)."@en.


############################################
# Properties of the highest-level concepts #
############################################

mso-em:isAssertedBy a owl:ObjectProperty;
   skos:prefLabel "is asserted by"@en;
   skos:altLabel  "isAssertedBy"@en;
   rdfs:domain mso-em:Claim;
   rdfs:range mso-em:Interlocutor;
   rdfs:subPropertyOf dol:generically-dependent-on;
   skos:definition "(x is asserted by y) means that x is a claim that is affirmatively communicated by the interlocutor y."@en.


#######################
# Subclasses of Claim #
#######################

mso-em:OwnClaim a owl:Class;
   skos:prefLabel "own claim"@en;
   skos:altLabel  "OwnClaim"@en;
   rdfs:subClassOf mso-em:Claim;
   owl:equivalentClass [
      a owl:Restriction;
      owl:onProperty mso-em:isAssertedBy;
      owl:someValuesFrom mso-em:Self
   ];
   skos:exactMatch pims-ii:OwnClaim;
   skos:definition "claim that is asserted by a self reference, i.e., held to be true by the present system"@en;
   skos:scopeNote "can be used to mark propositional content of the present knowledge base, as opposed to claims made by others"@en.


###############################
# Subclasses of Communication #
###############################

mso-em:ExpressiveAct a owl:Class;
   skos:prefLabel "expressive act"@en;
   skos:altLabel "ExpressiveAct"@en;
   rdfs:subClassOf mso-em:Communication, [
      a owl:Restriction;
      owl:onProperty mso-em:isDoneBy;
      owl:someValuesFrom mso-em:Interlocutor
   ];
   skos:exactMatch pims-ii:ExpressiveAct;
   skos:definition "elementary unit of communication done by its agent, the speaker"@en;
   skos:example "e.g., a speech act or an analogous digital act of communicating"@en;
   skos:scopeNote "The role of the speaker (agent doing the expressive act) must be understood in a generalized sense, i.e., not limited to speech. The purpose of the action consists in its illocutionary and perlocutionary intent."@en.
