
##########################
# MSO-EM agency ontology #
##########################

@base <https://www.purl.org/mso-em#>.
@prefix mso-em: <https://www.purl.org/mso-em#>.

@prefix dcelem: <http://purl.org/dc/elements/1.1/>.
@prefix dcterms: <http://purl.org/dc/terms/>.
@prefix dol: <http://www.loa-cnr.it/ontologies/DOLCE-Lite.owl#>.
@prefix ineurese: <http://purl.org/info:eu-repo/semantics/>.
@prefix pims-ii: <http://www.molmod.info/semantics/pims-ii.ttl#>.
@prefix vann: <http://purl.org/vocab/vann/>.
@prefix xs: <http://www.w3.org/2001/XMLSchema#>.

<https://www.purl.org/mso-em-agency> a owl:Ontology;
   owl:versionIRI <https://batcat.info/semantics/mso-em-2024-09/sign.ttl>;
   dcterms:title "MSO-EM module 'sign' (Articulation, Plurality, Structure)"^^xs:string;
   dcterms:created "2024"^^dcterms:W3CDTF;
   owl:versionInfo "MSO-EM module 'sign': Version dated September 2024"^^xs:string;
   dcterms:issued "2024-09-26"^^dcterms:W3CDTF;
   dcterms:publisher "BatCAT consortium (Horizon Europe GA no. 101137725)"^^xs:string;
   dcterms:license <https://creativecommons.org/licenses/by-nd/4.0/>;
   dcterms:creator <https://orcid.org/0000-0002-9464-6739>;  # Martin Thomas Horsch
   dcterms:status ineurese:publishedVersion;
   dcterms:source <http://www.molmod.info/semantics/pims-ii.ttl>;
   vann:preferredNamespaceUri "https://www.purl.org/mso-em#"^^xs:string;
   dcelem:description "MSO-EM module for signs. Its highest-level concepts are Articulation, Plurality, and Structure."@en;
   dcterms:bibliographicCitation "M. T. Horsch, S. Chiacchiera, I. T. Todorov, A. T. Correia, A. Dey, N. A. Konchakova, S. Scholze, S. Stephan, K. TÃ¸ndel, A. Sarkar, M. H. Karray, F. Al Machot, B. Schembera, 'Exploration of key concepts required for mid- and domain-level ontology development to facilitate explainable-AI-readiness of data and models,' submitted, 2024."@en.


##########################
# Highest-level concepts #
##########################

mso-em:Articulation a owl:Class;
   skos:prefLabel "Articulation"@en;
   rdfs:label     "Articulation"@en;
   skos:altLabel "Articulation"@en;
   rdfs:subClassOf dol:non-physical-endurant, [
      a owl:Restriction;
      owl:onProperty mso-em:isRealizedBy;
      owl:someValuesFrom dol:endurant
   ];
   skos:exactMatch pims-ii:Articulation;
   skos:definition "articulation (collective expression), i.e., a sign (type/collection) the realizations of which are not collective expressions, but individual literal (written or digital) or non-literal (e.g., spoken) items with the same semiotic function."@en.

mso-em:Plurality a owl:Class;
   skos:prefLabel "Plurality"@en;
   rdfs:label     "Plurality"@en;
   skos:altLabel "Plurality"@en;
   rdfs:subClassOf dol:abstract, [
      a owl:Restriction;
      owl:onProperty mso-em:hasElement;
      owl:someValuesFrom owl:Thing
   ];
   skos:exactMatch pims-ii:Plurality;
   owl:disjointWith [
      a owl:Restriction;
      owl:onProperty dol:specific-constant-constituent;
      owl:someValuesFrom mso-em:Plurality
   ], [
      a owl:Restriction;
      owl:onProperty dol:specific-constant-constituent;
      owl:someValuesFrom mso-em:Structure
   ];
   skos:definition "plurality, i.e., a tuple the members of which are a representational element (referent or representamen) together, whereby all act/contribute in the same way"@en;
   skos:example "The referent of the expression 'the four seasons/quarters of the year' (for a given year, within a given spatial region) is a plurality, and each of the four seasons/quarters is one of its semiotic members"@en.

mso-em:Structure a owl:Class;
   skos:prefLabel "Structure"@en;
   rdfs:label     "Structure"@en;
   skos:altLabel "Structure"@en;
   rdfs:subClassOf dol:abstract, [
      a owl:Restriction;
      owl:onProperty mso-em:hasElement;
      owl:someValuesFrom owl:Thing
   ];
   owl:disjointWith [
      a owl:Restriction;
      owl:onProperty dol:specific-constant-constituent;
      owl:someValuesFrom mso-em:Structure
   ];
   skos:exactMatch pims-ii:Structure;
   skos:definition "structure, i.e., a semiotic collective the semiotic members of which complement each other, contributing in different ways (or, at least, not all int the same way) to their joint action as a referent or a representamen"@en.


############################################
# Properties of the highest-level concepts #
############################################

mso-em:hasElement a owl:ObjectProperty;
   skos:prefLabel "has element"@en;
   rdfs:label     "has element"@en;
   rdfs:subPropertyOf dol:specific-constant-constituent;
   rdfs:domain dol:abstract;
   skos:definition "(x has element y) means that y is an entry in the plurality (tuple), structure, or set x"@en.

mso-em:isArticulatedBy a owl:ObjectProperty;
   skos:prefLabel "is articulated by"@en;
   rdfs:label     "is articulated by"@en;
   skos:altLabel "isArticulatedBy"@en;
   rdfs:subPropertyOf dol:generic-constituent;
   rdfs:domain dol:proposition;
   rdfs:range mso-em:Articulation;
   skos:definition "(y is articulated by x) means that x is a semiotic member of the proposition y, giving a literal or non-literal (e.g., spoken) expression to its propositional content; n.b., x may also express other propositions beside y"@en.
dol:proposition rdfs:subClassOf [
      a owl:Restriction;
      owl:onProperty mso-em:isArticulatedBy;
      owl:someValuesFrom mso-em:Articulation
   ].
   
mso-em:isRealizedBy a owl:ObjectProperty;
   skos:prefLabel "is realized by"@en;
   rdfs:label "is realized by"@en;
   skos:altLabel "isRealizedBy"@en;
   rdfs:subPropertyOf dol:generic-constituent;
   rdfs:domain mso-em:Articulation;
   rdfs:range dol:endurant;
   skos:definition "(y is realized by y) means that x, which is not a semiotic collective, is a literal or non-literal realization of the expression y"@en.
