########################
# MSO-EM sign ontology #
########################

@base <https://www.purl.org/mso-em#>.
@prefix mso-em: <https://www.purl.org/mso-em#>.

@prefix dcelem: <http://purl.org/dc/elements/1.1/>.
@prefix dcterms: <http://purl.org/dc/terms/>.
@prefix dol: <http://www.loa-cnr.it/ontologies/DOLCE-Lite.owl#>.
@prefix ineurese: <http://purl.org/info:eu-repo/semantics/>.
@prefix pims-ii: <http://www.molmod.info/semantics/pims-ii.ttl#>.
@prefix skos: <http://www.w3.org/2004/02/skos/core#>.
@prefix vann: <http://purl.org/vocab/vann/>.
@prefix xs: <http://www.w3.org/2001/XMLSchema#>.

<https://www.purl.org/mso-em-sign> a owl:Ontology;
   owl:versionIRI <https://batcat.info/semantics/mso-em-2025-07/sign.ttl>;
   dcterms:title "MSO-EM module 'sign' (Articulation, Plurality, Structure)"^^xs:string;
   dcterms:created "2024-2025"^^dcterms:W3CDTF;
   owl:versionInfo "MSO-EM module 'sign': Version dated July 2025"^^xs:string;
   dcterms:issued "2025-07-13"^^dcterms:W3CDTF;
   dcterms:publisher "BatCAT consortium (Horizon Europe GA no. 101137725)"^^xs:string;
   dcterms:license <https://creativecommons.org/licenses/by-nd/4.0/>;
   dcterms:creator <https://orcid.org/0000-0002-9464-6739>;  # Martin Thomas Horsch
   dcterms:status ineurese:publishedVersion;
   dcterms:source <http://www.molmod.info/semantics/pims-ii.ttl>;
   vann:preferredNamespaceUri "https://www.purl.org/mso-em#"^^xs:string;
   dcelem:description "MSO-EM module for signs. Its highest-level concepts are Articulation, Plurality, and Structure."@en;
   dcterms:bibliographicCitation "M. T. Horsch, S. Chiacchiera, I. T. Todorov, A. T. Correia, A. Dey, N. A. Konchakova, S. Scholze, S. Stephan, K. TÃ¸ndel, A. Sarkar, M. H. Karray, F. Al Machot, B. Schembera, 'Exploration of key concepts required for mid- and domain-level ontology development to facilitate explainable-AI-readiness of data and models,' submitted, 2024."@en.


##########################
# Highest-level concepts #
##########################

mso-em:Articulation a owl:Class;
   skos:prefLabel "articulation"@en;
   skos:altLabel  "Articulation"@en;
   rdfs:subClassOf dol:non-physical-endurant, [
      a owl:Restriction;
      owl:onProperty mso-em:isRealizedBy;
      owl:someValuesFrom dol:endurant
   ];
   skos:exactMatch pims-ii:Articulation;
   skos:definition "sign (type/collection) the realizations of which are not collective expressions, but individual literal (written or digital) or non-literal (e.g., spoken) items with the same semiotic function."@en.

mso-em:Plurality a owl:Class;
   skos:prefLabel "plurality"@en;
   skos:altLabel  "Plurality"@en;
   rdfs:subClassOf dol:abstract, [
      a owl:Restriction;
      owl:onProperty mso-em:hasElement;
      owl:someValuesFrom owl:Thing
   ];
   skos:exactMatch pims-ii:Plurality;
   owl:disjointWith dol:proposition, mso-em:Structure, [
      a owl:Restriction;
      owl:onProperty dol:specific-constant-constituent;
      owl:someValuesFrom mso-em:Plurality
   ], [
      a owl:Restriction;
      owl:onProperty dol:specific-constant-constituent;
      owl:someValuesFrom mso-em:Structure
   ];
   skos:definition "tuple the members of which are *one* representational element (referent or representamen) *together*, whereby all act/contribute in the same way"@en;
   skos:example "The referent of the expression 'the four seasons/quarters of the year' (for a given year, within a given spatial region) is a plurality, and each of the four seasons/quarters is one of its semiotic members."@en.

mso-em:Structure a owl:Class;
   skos:prefLabel "structure"@en;
   skos:altLabel  "Structure"@en;
   rdfs:subClassOf dol:abstract, [
      a owl:Restriction;
      owl:onProperty mso-em:hasElement;
      owl:someValuesFrom owl:Thing
   ];
   owl:disjointWith dol:proposition, mso-em:Plurality, [
      a owl:Restriction;
      owl:onProperty dol:specific-constant-constituent;
      owl:someValuesFrom mso-em:Structure
   ];
   skos:exactMatch pims-ii:Structure;
   skos:definition "semiotic collective the semiotic members of which complement each other, contributing in different ways (or, at least, not all int the same way) to their joint action as a referent or a representamen"@en.


############################################
# Properties of the highest-level concepts #
############################################

mso-em:hasElement a owl:ObjectProperty;
   skos:prefLabel "has element"@en;
   skos:altLabel  "hasElement"@en;
   rdfs:subPropertyOf dol:specific-constant-constituent;
   rdfs:domain dol:abstract;
   skos:definition "(x has element y) means that y is an element of the plurality (tuple), structure, or set x."@en;
   skos:scopeNote "also applied to the factors of a topical product (by analogy with the summands of a topical sum, which are elements of a plurality"@en.

mso-em:isArticulatedBy a owl:ObjectProperty;
   skos:prefLabel "is articulated by"@en;
   skos:altLabel  "isArticulatedBy"@en;
   rdfs:subPropertyOf dol:generic-constituent;
   rdfs:domain dol:proposition;
   rdfs:range mso-em:Articulation;
   skos:definition "(y is articulated by x) means that x is a semiotic member of the proposition y, giving a literal or non-literal (e.g., spoken) expression to its propositional content; n.b., x may also express other propositions beside y."@en.
dol:proposition rdfs:subClassOf [
      a owl:Restriction;
      owl:onProperty mso-em:isArticulatedBy;
      owl:someValuesFrom mso-em:Articulation
   ].
   
mso-em:isRealizedBy a owl:ObjectProperty;
   skos:prefLabel "is realized by"@en;
   skos:altLabel  "isRealizedBy"@en;
   rdfs:subPropertyOf dol:generic-constituent;
   rdfs:domain mso-em:Articulation;
   rdfs:range dol:endurant;
   skos:definition "(y is realized by y) means that x, which is not a semiotic collective, is a literal or non-literal realization of the expression y."@en.

   
##############################
# Subclasses of Articulation #
##############################

mso-em:DataItem a owl:Class;
   skos:prefLabel "data item"@en;
   skos:altLabel  "DataItem"@en;
   rdfs:subClassOf mso-em:Literal, [
      a owl:Restriction;
      owl:onProperty mso-em:hasEntry;
      owl:someValuesFrom mso-em:Literal
   ];
   owl:disjointWith mso-em:IRI, mso-em:Name;
   skos:exactMatch pims-ii:DataItem;
   skos:definition "digital articulation given as a tuple of literals"@en;
   skos:example "e.g., a key-value dyad with a left-hand side and a right-hand side"@en.

mso-em:Dataset a owl:Class;
   skos:prefLabel "dataset"@en;
   skos:altLabel  "Dataset"@en;
   rdfs:subClassOf mso-em:Articulation, [
      a owl:Restriction;
      owl:onProperty mso-em:hasEntry;
      owl:someValuesFrom mso-em:DataItem
   ];
   owl:disjointwith mso-em:Literal, mso-em:Utterance;
   skos:exactMatch pims-ii:Dataset;
   skos:definition "digital articulation that is composed of data items that are similar in shape, kind, and content type"@en.

mso-em:Dyad a owl:Class;
   skos:prefLabel "dyad"@en;
   skos:altLabel  "Dyad"@en;
   rdfs:subClassOf mso-em:DataItem, [
      a owl:Restriction;
      owl:onProperty mso-em:hasLeftEntry;
      owl:someValuesFrom mso-em:Articulation
   ], [
      a owl:Restriction;
      owl:onProperty mso-em:hasRightEntry;
      owl:someValuesFrom mso-em:Articulation
   ];
   owl:disjointWith mso-em:Triple;
   skos:exactMatch pims-ii:Dyad;
   skos:definition "data item by which two articulations are grouped together"@en;
   skos:example "e.g., an equality or inequality articulation"@en.

mso-em:IRI a owl:Class;
   skos:prefLabel "IRI"@en;
   skos:altLabel  "IRI"@en;
   rdfs:subClassOf mso-em:Literal;
   skos:exactMatch pims-ii:IRI;
   skos:definition "internationalized resource identifier (IRI) as defined by RFC 3987"@en;
   skos:scopeNote "an IRI object should be related by 'isLiterally' to an xs:string containing the IRI literal"@en.

mso-em:Literal a owl:Class;
   skos:prefLabel "literal"@en;
   skos:altLabel  "Literal"@en;
   rdfs:subClassOf mso-em:Articulation, [
      a owl:Restriction;
      owl:onProperty mso-em:isLiterally;
      owl:someValuesFrom rdfs:Literal
   ];
   owl:disjointWith mso-em:Dataset, mso-em:Utterance;
   skos:exactMatch pims-ii:CollectiveLiteral;
   skos:definition "semiotic collective the members of which all have a digital, printed, or written textual/numerical form in that they are all instances/copies of the same RDFS literal (or multiple RDFS literals that are very similar"@en;
   skos:example "different ways of spelling/abbreviating the same word or denoting the same number can be considered realizations of a single literal"@en.

mso-em:Name a owl:Class;
   skos:prefLabel "name"@en;
   skos:altLabel  "Name"@en;
   rdfs:subClassOf mso-em:Literal;
   skos:exactMatch pims-ii:Name;
   skos:definition "lexeme that acts as a rigid designator due to social convention"@en.

mso-em:Triple a owl:Class;
   skos:prefLabel "triple"@en;
   skos:altLabel  "Triple"@en;
   rdfs:subClassOf mso-em:DataItem, [
      a owl:Restriction;
      owl:onProperty mso-em:hasLeftEntry;
      owl:someValuesFrom mso-em:IRI
   ], [
      a owl:Restriction;
      owl:onProperty mso-em:hasMidEntry;
      owl:someValuesFrom mso-em:IRI
   ], [
      a owl:Restriction;
      owl:onProperty mso-em:hasRightEntry;
      owl:someValuesFrom mso-em:IRI
   ];
   owl:disjointWith mso-em:Dyad;
   skos:definition "subject-predicate-object triple (connected by relations to the IRIs of the subject, predicate, and object)"@en.

mso-em:Utterance a owl:Class;
   skos:prefLabel "utterance"@en;
   skos:altLabel  "Utterance"@en;
   rdfs:subClassOf mso-em:Articulation;
   owl:disjointWith mso-em:Dataset, mso-em:Literal;
   skos:exactMatch pims-ii:CollectiveUtterance;
   skos:definition "semiotic collective the members of which do not have digital, printed, or written textual/numerical form and the members of which are all attributed the same semantics and pragmatics"@en.


############################################
# Properties of subclasses of Articulation #
############################################

mso-em:hasEntry a owl:ObjectProperty;
   skos:prefLabel "has entry"@en;
   skos:altLabel  "hasEntry"@en;
   rdfs:subPropertyOf dol:specific-constant-constituent;
   rdfs:domain mso-em:Articulation;
   rdfs:range mso-em:Articulation;
   skos:definition "(x has entry y) means that x is an articulation and y, also an articulation, is one of its constitutive elements."@en.

mso-em:hasLeftEntry a owl:ObjectProperty;
   skos:prefLabel "has left entry"@en;
   skos:altLabel  "hasLeftEntry"@en;
   rdfs:subPropertyOf mso-em:hasEntry;
   skos:definition "(x has left entry y) means that x is an articulation with multiple entries, and y is the 'left' one."@en;
   skos:scopeNote "used for the subject entry of a mso-em:Triple and for the first element of a mso-em:Dyad"@en.

mso-em:hasMidEntry a owl:ObjectProperty;
   skos:prefLabel "has mid entry"@en;
   skos:altLabel  "hasMidEntry"@en;
   rdfs:subPropertyOf mso-em:hasEntry;
   skos:definition "(x has mid entry y) means that x is an articulation with multiple entries, and y is the 'mid' one."@en;
   skos:scopeNote "used for the predicate entry of a mso-em:Triple"@en.

mso-em:hasRightEntry a owl:ObjectProperty;
   skos:prefLabel "has right entry"@en;
   skos:altLabel  "hasLeftEntry"@en;
   rdfs:subPropertyOf mso-em:hasEntry;
   skos:definition "(x has right entry y) means that x is an articulation with multiple entries, and y is the 'right' one."@en;
   skos:scopeNote "used for the object entry of a mso-em:Triple and for the second element of a mso-em:Dyad"@en.

mso-em:isLiterally a owl:DatatypeProperty;
   skos:prefLabel "is literally"@en;
   skos:altLabel  "isLiterally"@en;
   rdfs:domain mso-em:Literal;
   skos:exactMatch pims-ii:isLiterally;
   skos:definition "points to the expression of a collective literal as an RDFS literal (e.g., xs:string or xs:decimal)"@en.

mso-em:isNameFor a owl:ObjectProperty;
   skos:prefLabel "is name for"@en;
   skos:altLabel  "isNameFor"@en;
   rdfs:domain mso-em:Name;
   rdfs:subPropertyOf mso-em:represents;
   skos:exactMatch pims-ii:isNameFor;
   skos:definition "(x isNameFor y), to be applied in the frequent special case where y is represented by x, its name"@en.

mso-em:represents a owl:ObjectProperty;
   skos:prefLabel "represents"@en;
   skos:altLabel "represents"@en;
   rdfs:subPropertyOf dol:generically-dependent-on;
   skos:exactMatch pims-ii:isRepresentamenFor;
   skos:definition "Dyadic representation relation; (x represents y) means that, in a Peircean sense, x is a sign (i.e., a representamen) for y"@en;
   skos:scopeNote "(x represents y) requires that there is a cognitive step z such that (x isRepresentamenIn z) and (y isReferentIn z)"@en.
