##############################
# MSO-EM simulation ontology #
##############################

@base <https://www.purl.org/mso-em#>.
@prefix mso-em: <https://www.purl.org/mso-em#>.

@prefix dcelem: <http://purl.org/dc/elements/1.1/>.
@prefix dcterms: <http://purl.org/dc/terms/>.
@prefix dol: <http://www.loa-cnr.it/ontologies/DOLCE-Lite.owl#>.
@prefix ineurese: <http://purl.org/info:eu-repo/semantics/>.
@prefix pims-ii: <http://www.molmod.info/semantics/pims-ii.ttl#>.
@prefix skos: <http://www.w3.org/2004/02/skos/core#>.
@prefix vann: <http://purl.org/vocab/vann/>.
@prefix xs: <http://www.w3.org/2001/XMLSchema#>.

<https://www.purl.org/mso-em-simulation> a owl:Ontology;
   owl:versionIRI <https://batcat.info/semantics/mso-em-2024-12/simulation.ttl>;
   dcterms:title "MSO-EM module 'simulation' (CompleteModel, Simulation, ...)"^^xs:string;
   dcterms:created "2024"^^dcterms:W3CDTF;
   owl:versionInfo "MSO-EM module 'simulation': Version dated December 2024"^^xs:string;
   dcterms:issued "2024-12-01"^^dcterms:W3CDTF;
   dcterms:publisher "BatCAT consortium (Horizon Europe GA no. 101137725)"^^xs:string;
   dcterms:license <https://creativecommons.org/licenses/by-nd/4.0/>;
   dcterms:creator <https://orcid.org/0000-0002-9464-6739>;  # Martin Thomas Horsch
   dcterms:status ineurese:publishedVersion;
   dcterms:source <http://www.molmod.info/semantics/pims-ii.ttl>;
   vann:preferredNamespaceUri "https://www.purl.org/mso-em#"^^xs:string;
   dcelem:description "MSO-EM module for simulation. Its highest-level concepts are CompleteModel, Simulation, ...."@en;
   dcterms:bibliographicCitation "M. T. Horsch, S. Chiacchiera, I. T. Todorov, A. T. Correia, A. Dey, N. A. Konchakova, S. Scholze, S. Stephan, K. TÃ¸ndel, A. Sarkar, M. H. Karray, F. Al Machot, B. Schembera, 'Exploration of key concepts required for mid- and domain-level ontology development to facilitate explainable-AI-readiness of data and models,' submitted, 2024."@en.


##########################
# Highest-level concepts #
##########################

mso-em:CompleteModel a owl:Class;
   skos:prefLabel "complete model"@en;
   skos:altLabel  "CompleteModel"@en;
   rdfs:subClassOf mso-em:Articulation, dol:non-physical-endurant;
   skos:definition "articulation consisting of a complete, determined set of equations that can be evaluated in a simulation without requiring any additional information"@en;
   skos:scopeNote "any endurant can serve as a model of something (typically it will be an articulation); this class is specifically for the finalized, complete set of equations, including the computational representation of the model and any additional information needed"@en.

mso-em:Simulation a owl:Class;
   skos:prefLabel "simulation"@en;
   skos:altLabel  "Simulation"@en;
   rdfs:subClassOf mso-em:Interpretation, dol:event, [
      a owl:Restriction;
      owl:onProperty mso-em:involvesSign;
      owl:someValuesFrom mso-em:Articulation
   ], [
      a owl:Restriction;
      owl:onProperty mso-em:involvesInterpretant;
      owl:someValuesFrom mso-em:Articulation
   ];
   owl:equivalentClass [
      a owl:Restriction;
      owl:onProperty mso-em:evaluatesModel;
      owl:someValuesFrom mso-em:CompleteModel
   ];
   skos:exactMatch pims-ii:Simulation;
   skos:definition "purposefully conducted numerical interpretation of simulation input (model, etc.), where the interpretant is the simulation result"@en.


############################################
# Properties of the highest-level concepts #
############################################

mso-em:evaluatesModel a owl:ObjectProperty;
   skos:prefLabel "evaluates model"@en;
   skos:altLabel "evaluatesModel"@en;
   rdfs:subPropertyOf dol:specific-constant-dependent;
   rdfs:domain mso-em:Simulation;
   skos:definition "(x evaluates model y) means that y is a model considered in simulation x."@en;
   skos:scopeNote "in principle, anything can serve as a model of something; a simulation particularly needs a complete model, expressing all the equations specifying the simulation, but other (e.g. partially specified) models can be related to the simulation through this relation as well"@en.

mso-em:articulatesModelOf a owl:ObjectProperty;
   skos:prefLabel "articulates model of"@en;
   skos:altLabel "articulatesModelOf"@en;
   rdfs:subPropertyOf mso-em:isAbout, dol:generically-dependent-on;
   rdfs:domain mso-em:Articulation;
   skos:definition "(x articulates model of y) means that the articulation x is a model of y"@en;
   skos:example "e.g., x is a molecular model of methane in digital form (e.g., a file containing the model), and y is a methane molecule, a system containing pure methane, or something similar that is being modelled"@en.

mso-em:isDoneBy a owl:ObjectProperty;
   skos:prefLabel "is done by"@en;
   skos:altLabel "isDoneBy"@en;
   rdfs:subPropertyOf dol:constant-participant;
   rdfs:domain mso-em:Action;
   rdfs:range mso-em:Agent;
   skos:definition "(x is done by y) means that y is the agent that conducts/undertakes the action x."@en;
   skos:scopeNote "An action is done by exactly one agent."@en.
